fix +-1, BB(5)=47,176,870 now

BB52Statement.v
@@ -61,12 +61,14 @@ Inductive Steps: TM->nat->ExecState->ExecState->Prop :=
   step tm st0 = Some st1 ->
   Steps tm (S n) st st1.
 
-Definition HaltsAt(tm:TM)(n:nat)(st:ExecState): Prop :=
-  exists st', Steps tm n st st' /\ step tm st' = None.
+Inductive HaltsAt(tm:TM): nat->ExecState->Prop :=
+| HaltsAt_intro n st:
+  (exists st', Steps tm n st st' /\ step tm st' = None) ->
+  HaltsAt tm (S n) st.
 
 End TM.
 
-Definition BB5 := 47176869%N.
+Definition BB5 := 47176870%N.
 
 Definition BB5_value_statement :=
   (forall tm n0, HaltsAt Σ tm n0 (InitES Σ Σ0) -> n0 <= N.to_nat BB5) /\
